Cleanup STLCMonadic.v

theories/STLCMonadic.v
@@ -1,282 +1,87 @@
 (* TODO: Proof Persistent_Env
-   TODO: Proof Persistent (without the ')
+   TODO: Use implicit argument def. of Persistent
    TODO: define infer for the other cases
-   TODO: read ch 5 in paper for refinement proof *)
+   TODO: Refinement proof of deep embedding *)
 
-
-
-   Require Import List.
+Require Import List.
 Import ListNotations.
 Require Import String.
 From MasterThesis Require Import
      Context.
 Import ctx.notations.
 
-Inductive ty : Type :=
-  | ty_bool : ty
-  | ty_func : ty -> ty -> ty.
+Section Shallow.
 
-Inductive Ty (Σ : Ctx nat) : Type :=
-  | Ty_bool : Ty Σ
-  | Ty_func : Ty Σ -> Ty Σ -> Ty Σ
-  | Ty_hole : forall (i : nat), i ∈ Σ -> Ty Σ.
+  Inductive ty : Type :=
+    | ty_bool : ty
+    | ty_func : ty -> ty -> ty.
 
-Inductive expr : Type :=
-  (* values *)
-  | v_true  : expr
-  | v_false : expr
-  (* compound expressions *)
-  | e_if    : expr -> expr -> expr -> expr
-  | e_var   : string -> expr
-  | e_absu  : string -> expr -> expr
-  | e_abst  : string -> ty -> expr -> expr
-  | e_app   : expr -> expr -> expr.
+  Inductive expr : Type :=
+    (* values *)
+    | v_true  : expr
+    | v_false : expr
+    (* compound expressions *)
+    | e_if    : expr -> expr -> expr -> expr
+    | e_var   : string -> expr
+    | e_absu  : string -> expr -> expr
+    | e_abst  : string -> ty -> expr -> expr
+    | e_app   : expr -> expr -> expr.
 
-Definition env := list (string * ty).
-Definition Env Σ := list (string * Ty Σ).
+  Definition env := list (string * ty).
 
-Inductive Cstr (A : Ctx nat -> Type) (Σ : Ctx nat) : Type :=
-  | C_eqc : Ty Σ -> Ty Σ -> Cstr A Σ -> Cstr A Σ
-  | C_val : A Σ -> Cstr A Σ
-  | C_fls : Cstr A Σ
-  | C_exi : forall (i : nat), Cstr A (Σ ▻ i) -> Cstr A Σ.
-
-Check Cstr.
-
-Check Ty.
-
-Check Ty_bool.
-
-Check C_fls Ty.
-
-(* Adapted from Katamaran: Symbolic/Worlds.v *)
-
-Inductive Accessibility (Σ₁ : Ctx nat) : Ctx nat -> Type :=
-  | refl    : Accessibility Σ₁ Σ₁
-  | fresh α : forall Σ₂, Accessibility Σ₁ Σ₂ -> Accessibility Σ₁ (Σ₂ ▻ α).
-
-(* ⊢ A *)
-Definition Valid (A : Ctx nat -> Type) := forall Σ, A Σ.
-
-(* A → B *)
-Definition Impl (A B : Ctx nat -> Type) : Ctx nat -> Type :=
-  fun Σ => (A Σ) -> (B Σ).
-
-(* □ A *)
-Definition Box A (Σ : Ctx nat) := forall Σ', Accessibility Σ Σ' -> A Σ'.
-
-(* _[_] *)
-Definition Persistent' : Valid (Impl Ty (Box Ty)).
-Proof. cbv in *. intros. Admitted.
-
-Definition Persistent_Env : Valid (Impl Env (Box Env)).
-Admitted.
-
-Fixpoint Persistent {Σ₁ Σ₂} (t : Ty Σ₁) {w : Accessibility Σ₁ Σ₂} {struct t} : Ty Σ₂.
-Proof. cbv in *. intros. destruct t eqn:?.
-  - apply Ty_bool.
-  - constructor 2;
-    eapply Persistent. apply t0_1. apply w. apply t0_2. apply w.
-  - constructor 3 with i. admit.
-Show Proof. (* Defined, not Qed *)
-Admitted.
-
-Definition Persistent'' : Valid (Impl Ty (Box Ty)) :=
-  fun w0 x w1 ω01 =>
-    match ω01 with
-    | refl _ => x
-    | fresh _ α Σ _ => Ty_bool (Σ ▻ α)
+  Fixpoint value {X: Type} (var : string) (ctx : list (string * X)) : option X :=
+    match ctx with
+    | nil => None
+    | (var', val) :: ctx' =>
+        if (string_dec var var') then Some val else (value var ctx')
     end.
 
-Definition T {A} := fun (Σ : Ctx nat) (a : Box A Σ) => a Σ (refl Σ).
+  Reserved Notation "G |-- E ; T ~> EE"
+              (at level 50).
 
-Check T.
+  Inductive tpb : env -> expr -> ty -> expr -> Prop :=
+    | tpb_false : forall g,
+        g |-- v_false ; ty_bool ~> v_false
+    | tpb_true : forall g,
+        g |-- v_true ; ty_bool ~> v_true
+    | tpb_if : forall g cnd cnd' coq coq' alt alt' t,
+        g |-- cnd ; ty_bool ~> cnd' ->
+        g |-- coq ; t       ~> coq' ->
+        g |-- alt ; t       ~> alt' ->
+        g |-- (e_if cnd coq alt) ; t ~> (e_if cnd' coq' alt')
+    | tpb_var : forall g v vt,
+        value v g = Some vt ->
+        g |-- (e_var v) ; vt ~> (e_var v)
+    | tpb_absu : forall v vt g e e' t,
+        ((v, vt) :: g) |-- e ; t ~> e' ->
+        g |-- (e_absu v e) ; (ty_func vt t) ~> (e_abst v vt e')
+    | tpb_abst : forall v vt g e e' t,
+        ((v, vt) :: g) |-- e ; t ~> e' ->
+        g |-- (e_abst v vt e) ; (ty_func vt t) ~> (e_abst v vt e')
+    | tpb_app : forall g e1 t1 e1' e2 t2 e2',
+        g |-- e1 ; (ty_func t2 t1) ~> e1' ->
+        g |-- e2 ; t2 ~> e2' ->
+        g |-- (e_app e1 e2) ; t1 ~> (e_app e1' e2')
 
-Definition trans {Σ₁ Σ₂ Σ₃} (w12 : Accessibility Σ₁ Σ₂) (w23 : Accessibility Σ₂ Σ₃) : Accessibility Σ₁ Σ₃.
-Proof. induction w23. apply w12. apply fresh. apply IHw23. Defined.
+    where "G |-- E ; T ~> EE" := (tpb G E T EE).
 
-Definition _4 {A} : Valid (Impl (Box A) (Box (Box A))).
-Proof. cbv in *. intros.  apply X. eapply trans. apply H. apply H0. Show Proof. Defined.
+  Example ex_typing1 :
+    nil |-- (e_abst "x" ty_bool (e_var "x")) ; (ty_func ty_bool ty_bool) ~> (e_abst "x" ty_bool (e_var "x")).
+  Proof.
+    apply tpb_abst. apply tpb_var. cbn. reflexivity.
+  Qed.
 
-Check _4.
+  Example ex_typing2 :
+    nil |-- (e_absu "x" (e_var "x")) ; (ty_func ty_bool ty_bool) ~> (e_abst "x" ty_bool (e_var "x")).
+  Proof.
+    apply tpb_absu. apply tpb_var. cbn. reflexivity.
+  Qed.
 
-Print Scopes.
-
-Fixpoint value {X: Type} (var : string) (ctx : list (string * X)) : option X :=
-  match ctx with
-  | nil => None
-  | (var', val) :: ctx' =>
-      if (string_dec var var') then Some val else (value var ctx')
-  end.
-
-Fixpoint bind [A B] {Σ} (m : Cstr A Σ) (f : Box (Impl A (Cstr B)) Σ) {struct m} : Cstr B Σ.
-refine (
-  match m with
-  | C_eqc _ _ t1 t2 C1 => _
-  | C_val _ _ v => _
-  | C_fls _ _ => C_fls _ _ (* we just fail *)
-  | C_exi _ _ i C => _
-  end).
-Proof.
-  - apply C_eqc. apply t1. apply t2. eapply bind.
-    + apply C1.
-    + apply f.
-  - apply T in f. unfold Impl in f. apply f. apply v.
-  - eapply C_exi. eapply bind.
-    + apply C.
-    + apply _4 in f. cbv in *. intros. apply (f _ (fresh _ _ _ (refl Σ)) _ H X).
-Show Proof.
-Defined.
-
-Eval cbv [bind] in @bind.
-
-    Local Notation "[ ω ] x <- ma ;; mb" :=
-      (bind ma (fun _ ω x => mb))
-        (at level 80, x at next level,
-          ma at next level, mb at level 200,
-          right associativity).
-
-Definition Unit (Σ : Ctx nat) := unit.
-
-Check Unit.
-
-Definition assert {Σ} t1 t2 := C_eqc Unit Σ t1 t2 (C_val Unit Σ tt). (* TODO *)
-
-Fixpoint infer' {Σ} (Γ : Env Σ) (expression : expr) : Cstr Ty Σ :=
-  match expression with
-  | v_true => C_val Ty Σ (Ty_bool Σ)
-  | v_false => C_val Ty Σ (Ty_bool Σ)
-  | e_if cnd coq alt =>
-      [ ω₁ ] t_cnd <- infer' Γ cnd ;; (*
-      [ ω₂ ] t_coq <- infer' Γ coq ;;
-      [ ω₃ ] t_alt <- infer' Γ alt ;; *)
-      [ ω₄ ] _ <- assert t_cnd (Ty_bool _) ;;
-       (* [ ω₅ ] _ <- assert t_coq t_alt ;; *)
-      C_val Ty _ (@Persistent _ _ t_cnd ω₄)
-  | _ => C_fls Ty Σ
-  end.
-
-Check Persistent_Env.
-
-Fixpoint infer'' {Σ} (Γ : Env Σ) (expression : expr) : Cstr Ty Σ :=
-  match expression with
-  | v_true => C_val Ty Σ (Ty_bool Σ)
-  | v_false => C_val Ty Σ (Ty_bool Σ)
-  | e_if cnd coq alt =>
-      [ ω₁ ] t_cnd <- infer'' Γ cnd ;;
-      [ ω₂ ] t_coq <- infer'' ((Persistent_Env _ Γ) _ ω₁) coq ;; (* needs even more PERSISTENCY!!!, find where to persist ω₂ from Σ -> \c0 *)
-      [ ω₃ ] t_alt <- infer'' Γ alt ;; (* TODO: lift Γ into right world *)
-      [ ω₄ ] _ <- assert ((Persistent' _ t_cnd) _ ω₂) (Ty_bool _) ;;
-      [ ω₅ ] _ <- assert (Persistent t_coq) (Persistent t_alt) ;;
-         C_val Ty _ (Persistent t_coq) *)
-      C_fls Ty _
-  | _ => C_fls Ty Σ
-  end.
-
-Compute infer' nil (e_if v_true v_true v_false).
-Compute C_eqc Ty ε (Ty_bool ε) (Ty_bool ε) (C_val Ty ε (Ty_bool ε)).
-
-Reserved Notation "G |-- E ; T ~> EE"
-            (at level 50).
-
-Inductive tpb : env -> expr -> ty -> expr -> Prop :=
-  | tpb_false : forall g,
-      g |-- v_false ; ty_bool ~> v_false
-  | tpb_true : forall g,
-      g |-- v_true ; ty_bool ~> v_true
-  | tpb_if : forall g cnd cnd' coq coq' alt alt' t,
-      g |-- cnd ; ty_bool ~> cnd' ->
-      g |-- coq ; t       ~> coq' ->
-      g |-- alt ; t       ~> alt' ->
-      g |-- (e_if cnd coq alt) ; t ~> (e_if cnd' coq' alt')
-  | tpb_var : forall g v vt,
-      value v g = Some vt ->
-      g |-- (e_var v) ; vt ~> (e_var v)
-  | tpb_absu : forall v vt g e e' t, (* don't we have to come up with vt ? *)
-      (cons (v, vt) g) |-- e ; t ~> e' ->
-                   g |-- (e_absu v e) ; (ty_func vt t) ~> (e_abst v vt e')
-  | tpb_abst : forall v vt g e e' t,
-      (cons (v, vt) g) |-- e ; t ~> e' ->
-                   g |-- (e_abst v vt e) ; (ty_func vt t) ~> (e_abst v vt e')
-  | tpb_app : forall g e1 t1 e1' e2 t2 e2',
-      g |-- e1 ; (ty_func t2 t1) ~> e1' ->
-      g |-- e2 ; t2 ~> e2' ->
-      g |-- (e_app e1 e2) ; t1 ~> (e_app e1' e2')
-
-  where "G |-- E ; T ~> EE" := (tpb G E T EE).
-
-Example ex_typing1 :
-  nil |-- (e_abst "x" ty_bool (e_var "x")) ; (ty_func ty_bool ty_bool) ~> (e_abst "x" ty_bool (e_var "x")).
-Proof.
-  apply tpb_abst. apply tpb_var. cbn. reflexivity.
-Qed.
-
-Example ex_typing2 :
-  nil |-- (e_absu "x" (e_var "x")) ; (ty_func ty_bool ty_bool) ~> (e_abst "x" ty_bool (e_var "x")).
-Proof.
-  apply tpb_absu. apply tpb_var. cbn. reflexivity.
-Qed.
-
-Fixpoint gensem (ctx : list (string * ty)) (expression : expr) (type : ty) : Prop :=
-  match expression with
-  | v_true  => type = ty_bool
-  | v_false => type = ty_bool
-  | e_if cnd coq alt =>
-      gensem ctx cnd ty_bool /\
-      gensem ctx coq type    /\
-      gensem ctx alt type
-  | e_var var =>
-      match (value var ctx) with
-      | None => False
-      | Some t => t = type
-      end
-  | e_app e1 e2 =>
-      exists t2,
-      gensem ctx e1 (ty_func t2 type) /\
-      gensem ctx e2 t2
-  | e_absu var e =>
-      exists t_e t_var,
-      gensem ((var, t_var) :: ctx) e t_e /\
-      type = (ty_func t_var t_e)
-  | e_abst var t_var e =>
-      exists t_e,
-      gensem ((var, t_var) :: ctx) e t_e /\
-      type = (ty_func t_var t_e)
-  end.
-
-Lemma ex_gensem1 :
-  gensem nil (e_app (e_absu "x" (e_var "x")) v_false) ty_bool.
-Proof.
-  compute. repeat eexists.
-Qed.
-
-Example ex_gensem2 :
-gensem nil (e_app (e_absu "x" (v_true)) (e_absu "x" (e_var "x"))) ty_bool.
-Proof.
-  compute. repeat eexists.
-  Unshelve. apply ty_bool.
-Qed.
-
-Inductive freeM (A : Type) : Type :=
-  | bind_assert_free : ty -> ty -> freeM A -> freeM A
-  | ret_free : A -> freeM A
-  | fail_free : freeM A
-  | bind_exists_free : (ty -> freeM A) -> freeM A.
-
-(* PROOF MODE EXAMPLE *)
-
-(*
-Fixpoint freeM_bind [T1 T2 : Type] (m : freeM T1) (f : T1 -> freeM T2) {struct m} : freeM T2.
-refine (
-  match m with
-  | ret_free _ a => f a
-  | fail_free _ => fail_free T2
-  | bind_assert_free _ t1 t2 k =>
-      bind_assert_free _ t1 t2 (freeM_bind _ _ k f)
-  | bind_exists_free _ tf => _
-      (* bind_exists_free _ (fun t => freeM_bind (tf t) f) *)
-  end). apply bind_exists_free. intros t. eapply freeM_bind. apply (tf t). apply f.
-Show Proof. *)
+  Inductive freeM (A : Type) : Type :=
+    | bind_assert_free : ty -> ty -> freeM A -> freeM A
+    | ret_free : A -> freeM A
+    | fail_free : freeM A
+    | bind_exists_free : (ty -> freeM A) -> freeM A.
 
 Fixpoint freeM_bind [T1 T2 : Type] (m : freeM T1) (f : T1 -> freeM T2) : freeM T2 :=
    match m with
@@ -288,81 +93,60 @@ Fixpoint freeM_bind [T1 T2 : Type] (m : freeM T1) (f : T1 -> freeM T2) : freeM T
        bind_exists_free T2 (fun t : ty => freeM_bind (tf t) f)
    end.
 
-(*
-Inductive freeM (A : Type) : Type :=
-  | ret_free : A -> freeM A
-  | fail_free : freeM A
-  | bind_assert_free : ty -> ty -> freeM A -> freeM A
-  | bind_exists_free : freeM A -> freeM A.
+  Definition assert (t1 t2 : ty) := bind_assert_free _ t1 t2 (ret_free _ tt).
+  Definition exists_ty : freeM ty := bind_exists_free _ (fun t => ret_free _ t).
+  Definition ret [A : Type] (a : A) := ret_free A a.
+  Definition fail {A : Type} := fail_free A.
 
-Fixpoint freeM_bind [T1 T2 : Type] (m : freeM T1) (f : T1 -> freeM T2) : freeM T2 :=
-  match m with
-  | ret_free _ a => f a
-  | fail_free _ => fail_free T2
-  | bind_assert_free _ t1 t2 k =>
-      bind_assert_free _ t1 t2 (freeM_bind k f)
-  | bind_exists_free _ k =>
-      bind_exists_free _ (freeM_bind k f)
-  end.
-
- *)
-
-Definition assert (t1 t2 : ty) := bind_assert_free _ t1 t2 (ret_free _ tt).
-Check assert.
-Definition magic : freeM ty := bind_exists_free _ (fun t => ret_free _ t).
-Check magic.
-Definition ret [A : Type] (a : A) := ret_free A a.
-Definition fail {A : Type} := fail_free A.
-
-Notation "x <- ma ;; mb" :=
-        (freeM_bind ma (fun x => mb))
-          (at level 80, ma at next level, mb at level 200, right associativity).
-Notation "ma ;; mb" := (freeM_bind ma (fun _ => mb)) (at level 80, right associativity).
-Notation "' x <- ma ;; mb" :=
-        (freeM_bind ma (fun x => mb))
-          (at level 80, x pattern, ma at next level, mb at level 200, right associativity,
-           format "' x  <-  ma  ;;  mb").
+  Notation "x <- ma ;; mb" :=
+          (freeM_bind ma (fun x => mb))
+            (at level 80, ma at next level, mb at level 200, right associativity).
+  Notation "ma ;; mb" := (freeM_bind ma (fun _ => mb)) (at level 80, right associativity).
+  Notation "' x <- ma ;; mb" :=
+          (freeM_bind ma (fun x => mb))
+            (at level 80, x pattern, ma at next level, mb at level 200, right associativity,
+             format "' x  <-  ma  ;;  mb").
 
 
-Fixpoint infer (ctx : env) (expression : expr) : freeM (prod ty expr) :=
-  match expression with
-  | v_false => ret (ty_bool, expression)
-  | v_true  => ret (ty_bool, expression)
-  | e_if cnd coq alt =>
-      '(t_cnd, e_cnd) <- infer ctx cnd ;;
-      '(t_coq, e_coq) <- infer ctx coq ;;
-      '(t_alt, e_alt) <- infer ctx alt ;;
-      (assert t_cnd ty_bool) ;;
-      (assert t_coq t_alt)   ;;
-      ret (t_coq, e_if e_cnd e_coq e_alt)
-  | e_var var =>
-      match (value var ctx) with
-      | Some t_var => ret (t_var, expression)
-      | None => fail
-      end
-  | e_app e1 e2 =>
-      '(t_e1, e_e1) <- infer ctx e1 ;;
-      '(t_e2, e_e2) <- infer ctx e2 ;;
-      t_magic <- magic ;;
-      (assert t_e1 (ty_func t_e2 t_magic)) ;;
-      ret (t_magic, e_app e_e1 e_e2)
-  | e_absu var e =>
-      t_var <- magic ;;
-      '(t_e, e_e) <- infer (cons (var, t_var) ctx) e ;;
-      ret (ty_func t_var t_e, e_abst var t_var e_e)
-  | e_abst var t_var e =>
-      '(t_e, e_e) <- infer (cons (var, t_var) ctx) e ;;
-      ret (ty_func t_var t_e, e_abst var t_var e_e)
-  end.
+  Fixpoint infer (ctx : env) (expression : expr) : freeM (prod ty expr) :=
+    match expression with
+    | v_false => ret (ty_bool, expression)
+    | v_true  => ret (ty_bool, expression)
+    | e_if cnd coq alt =>
+        '(t_cnd, e_cnd) <- infer ctx cnd ;;
+        '(t_coq, e_coq) <- infer ctx coq ;;
+        '(t_alt, e_alt) <- infer ctx alt ;;
+        (assert t_cnd ty_bool) ;;
+        (assert t_coq t_alt)   ;;
+        ret (t_coq, e_if e_cnd e_coq e_alt)
+    | e_var var =>
+        match (value var ctx) with
+        | Some t_var => ret (t_var, expression)
+        | None => fail
+        end
+    | e_app e1 e2 =>
+        '(t_e1, e_e1) <- infer ctx e1 ;;
+        '(t_e2, e_e2) <- infer ctx e2 ;;
+        t_exists_ty <- exists_ty ;;
+        (assert t_e1 (ty_func t_e2 t_exists_ty)) ;;
+        ret (t_exists_ty, e_app e_e1 e_e2)
+    | e_absu var e =>
+        t_var <- exists_ty ;;
+        '(t_e, e_e) <- infer (cons (var, t_var) ctx) e ;;
+        ret (ty_func t_var t_e, e_abst var t_var e_e)
+    | e_abst var t_var e =>
+        '(t_e, e_e) <- infer (cons (var, t_var) ctx) e ;;
+        ret (ty_func t_var t_e, e_abst var t_var e_e)
+    end.
 
 Compute (infer nil (e_app (e_abst "x" ty_bool (e_var "x")) v_true)).
 Compute (infer nil (e_app (e_absu "x" (e_var "x")) v_true)).
 
-Definition K := (e_absu "k" (e_absu "l" (e_var "k"))).
+Definition K1 := (e_absu "k1" (e_absu "l" (e_var "k1"))).
+Definition K2 := (e_absu "k2" (e_absu "l" (e_var "k2"))).
 Definition I := (e_absu "i" (e_var "i")).
-Compute (infer nil K).
-Compute (infer nil I).
-Definition KKI := (e_app K (e_app K I)).
+
+Definition KKI := (e_app K1 (e_app K2 I)).
 Compute (infer nil KKI).
 
 
@@ -384,119 +168,273 @@ Fixpoint wp_freeM [A : Type] (m : freeM A) (Q: A -> Prop) :=
   | bind_exists_free _ tf => exists t : ty, wp_freeM (tf t) Q
   end.
 
-Lemma wlp_ty_eqb : forall (t1 t2 : ty) (Q : unit -> Prop),
-  wlp_freeM (assert t1 t2) Q <-> (t1 = t2 -> Q tt).
-Proof.
-  destruct t1, t2; cbn; intuition discriminate.
-Qed.
+  Lemma wlp_ty_eqb : forall (t1 t2 : ty) (Q : unit -> Prop),
+    wlp_freeM (assert t1 t2) Q <-> (t1 = t2 -> Q tt).
+  Proof.  destruct t1, t2; cbn; intuition discriminate.  Qed.
 
-Lemma wlp_exists_type : forall (Q: ty -> Prop),
-  wlp_freeM (magic) Q <-> (forall t : ty, Q t).
-Proof.
-  intuition.
-Qed.
+  Lemma wlp_exists_type : forall (Q: ty -> Prop),
+    wlp_freeM (exists_ty) Q <-> (forall t : ty, Q t).
+  Proof.  intuition.  Qed.
 
-Lemma wlp_bind : forall {A B : Type} (m1 : freeM A) (m2 : A -> freeM B) (Q : B -> Prop),
-  wlp_freeM (freeM_bind m1 m2) Q <-> wlp_freeM m1 (fun o => wlp_freeM (m2 o) Q).
-Proof.
-  split; induction m1; cbn; intuition; destruct H0; exists x; intuition.
-Qed.
+  Lemma wlp_bind : forall {A B : Type} (m1 : freeM A) (m2 : A -> freeM B) (Q : B -> Prop),
+    wlp_freeM (freeM_bind m1 m2) Q <-> wlp_freeM m1 (fun o => wlp_freeM (m2 o) Q).
+  Proof.  split; induction m1; cbn; intuition; destruct H0; exists x; intuition.  Qed.
 
-Lemma wlp_ret : forall {A : Type} (a : A) (Q : A -> Prop),
-  wlp_freeM (ret a) Q <-> Q a.
-Proof.
-  intuition.
-Qed.
+  Lemma wlp_ret : forall {A : Type} (a : A) (Q : A -> Prop),
+    wlp_freeM (ret a) Q <-> Q a.
+  Proof.  intuition.  Qed.
 
-Lemma wlp_fail : forall {A : Type} (Q : A -> Prop),
-  wlp_freeM (fail) Q <-> True.
-Proof.
-  intuition.
-Qed.
+  Lemma wlp_fail : forall {A : Type} (Q : A -> Prop),
+    wlp_freeM (fail) Q <-> True.
+  Proof.  intuition.  Qed.
 
-Lemma wlp_monotone : forall {O : Set} (P Q : O -> Prop) (m : freeM O),
-  (forall o : O, P o -> Q o) -> wlp_freeM m P -> wlp_freeM m Q.
-Proof.
-  intros. induction m; cbn; auto.
-Qed.
+  Lemma wlp_monotone : forall {O : Set} (P Q : O -> Prop) (m : freeM O),
+    (forall o : O, P o -> Q o) -> wlp_freeM m P -> wlp_freeM m Q.
+  Proof.  intros. induction m; cbn; auto.  Qed.
 
-Lemma wp_ty_eqb : forall (t1 t2 : ty) (Q : unit -> Prop),
-  wp_freeM (assert t1 t2) Q <-> t1 = t2 /\ Q tt.
-Proof.
-    split; intros.
-    - inversion H. cbn in H1. auto.
-    - cbn. apply H.
-Qed.
+  Lemma wp_ty_eqb : forall (t1 t2 : ty) (Q : unit -> Prop),
+    wp_freeM (assert t1 t2) Q <-> t1 = t2 /\ Q tt.
+  Proof.
+      split; intros.
+      - inversion H. cbn in H1. auto.
+      - cbn. apply H.
+  Qed.
 
-Lemma wp_exists_type : forall (Q: ty -> Prop),
-  wp_freeM (magic) Q <-> (exists t : ty, Q t).
-Proof.
-  intuition.
-Qed.
+  Lemma wp_exists_type : forall (Q: ty -> Prop),
+    wp_freeM (exists_ty) Q <-> (exists t : ty, Q t).
+  Proof.  intuition.  Qed.
 
-Lemma wp_bind : forall {A B : Type} (m1 : freeM A) (m2 : A -> freeM B) (Q : B -> Prop),
-  wp_freeM (freeM_bind m1 m2) Q <-> wp_freeM m1 (fun o => wp_freeM (m2 o) Q).
-Proof.
-    split; induction m1; cbn; intuition; destruct H0; exists x; intuition.
-Qed.
+  Lemma wp_bind : forall {A B : Type} (m1 : freeM A) (m2 : A -> freeM B) (Q : B -> Prop),
+    wp_freeM (freeM_bind m1 m2) Q <-> wp_freeM m1 (fun o => wp_freeM (m2 o) Q).
+  Proof.  split; induction m1; cbn; intuition; destruct H0; exists x; intuition.  Qed.
 
-Lemma wp_ret : forall {A : Type} (a : A) (Q : A -> Prop),
-  wp_freeM (ret a) Q <-> Q a.
-Proof.
-  intuition.
-Qed.
+  Lemma wp_ret : forall {A : Type} (a : A) (Q : A -> Prop),
+    wp_freeM (ret a) Q <-> Q a.
+  Proof.  intuition.  Qed.
 
-Lemma wp_fail : forall {A : Type} (Q : A -> Prop),
-  wp_freeM (fail) Q <-> False.
-Proof.
-  cbn. intuition.
-Qed.
+  Lemma wp_fail : forall {A : Type} (Q : A -> Prop),
+    wp_freeM (fail) Q <-> False.
+  Proof.  cbn. intuition.  Qed.
 
-Lemma wp_monotone : forall {O : Set} (P Q : O -> Prop) (m : freeM O),
-  (forall o : O, P o -> Q o) -> wp_freeM m P -> wp_freeM m Q.
-Proof.
-    intros. induction m; cbn; auto;
-    inversion H0; intuition.
-    exists x. apply H1. apply H2.
-Qed.
+  Lemma wp_monotone : forall {O : Set} (P Q : O -> Prop) (m : freeM O),
+    (forall o : O, P o -> Q o) -> wp_freeM m P -> wp_freeM m Q.
+  Proof.
+      intros. induction m; cbn; auto;
+      inversion H0; intuition.
+      exists x. apply H1. apply H2.
+  Qed.
 
 
-Lemma infer_sound : forall (G : env) (e : expr),
- wlp_freeM (infer G e) (fun '(t,ee) => G |-- e ; t ~> ee).
-Proof.
-  intros. generalize dependent G. induction e; cbn [infer]; intro;
-  repeat (rewrite ?wlp_exists_type, ?wlp_bind, ?wlp_ty_eqb, ?wlp_ret, ?wlp_fail; try destruct o;
-      try match goal with
-      | IHe : forall G, wlp_freeM (infer G ?e) _ |- wlp_freeM (infer ?g ?e) _ =>
-          specialize (IHe g); revert IHe; apply wlp_monotone; intros
-      | |- tpb _ _ _ _ =>
-          constructor
-      | |- ?x = ?y -> _ =>
-          intro; subst
-      | |- wlp_freeM (match ?t with _ => _ end) _ =>
-          destruct t eqn:?
-      | |- forall t, _ =>
-          intro
-      | H : ?g |-- ?e ; ?t ~> ?ee |- ?g' |-- e_app ?e1 ?e2 ; ?t' ~> e_app ?e1' ?e2' =>
-          apply (tpb_app _ _ _ _ _ t0 _)
-      end; try reflexivity; try assumption).
-Qed.
+  Lemma infer_sound : forall (G : env) (e : expr),
+   wlp_freeM (infer G e) (fun '(t,ee) => G |-- e ; t ~> ee).
+  Proof.
+    intros. generalize dependent G. induction e; cbn [infer]; intro;
+    repeat (rewrite ?wlp_exists_type, ?wlp_bind, ?wlp_ty_eqb, ?wlp_ret, ?wlp_fail; try destruct o;
+        try match goal with
+        | IHe : forall G, wlp_freeM (infer G ?e) _ |- wlp_freeM (infer ?g ?e) _ =>
+            specialize (IHe g); revert IHe; apply wlp_monotone; intros
+        | |- tpb _ _ _ _ =>
+            constructor
+        | |- ?x = ?y -> _ =>
+            intro; subst
+        | |- wlp_freeM (match ?t with _ => _ end) _ =>
+            destruct t eqn:?
+        | |- forall t, _ =>
+            intro
+        | H : ?g |-- ?e ; ?t ~> ?ee |- ?g' |-- e_app ?e1 ?e2 ; ?t' ~> e_app ?e1' ?e2' =>
+            apply (tpb_app _ _ _ _ _ t0 _)
+        end; try reflexivity; try assumption).
+  Qed.
 
-Lemma infer_complete : forall  (G : env) (e ee : expr) (t : ty),
-  (G |-- e ; t ~> ee) -> wp_freeM (infer G e) (fun '(t',ee')  => t = t' /\ ee = ee').
-Proof.
-  intros. induction H; cbn;
-  repeat (rewrite ?wp_bind, ?wp_ty_eqb, ?wp_ret, ?wp_fail; try destruct o; cbn; try rewrite H;
-      try match goal with
-      | IH : wp_freeM (infer ?g ?e) _ |- wp_freeM (infer ?g ?e) _ =>
-          revert IH; apply wp_monotone; intros; subst
-      | |- ?x = ?y /\ _ =>
-          split
-      | H : ?x = ?y /\ _ |- _ =>
-          destruct H; subst
-      end; try reflexivity).
-      - exists vt. apply wp_bind. revert IHtpb. apply wp_monotone. intro. destruct o. intro. destruct H0. apply wp_ret. subst. intuition.
-      - exists t1. auto.
-Qed.
+  Lemma infer_complete : forall  (G : env) (e ee : expr) (t : ty),
+    (G |-- e ; t ~> ee) -> wp_freeM (infer G e) (fun '(t',ee')  => t = t' /\ ee = ee').
+  Proof.
+    intros. induction H; cbn;
+    repeat (rewrite ?wp_bind, ?wp_ty_eqb, ?wp_ret, ?wp_fail; try destruct o; cbn; try rewrite H;
+        try match goal with
+        | IH : wp_freeM (infer ?g ?e) _ |- wp_freeM (infer ?g ?e) _ =>
+            revert IH; apply wp_monotone; intros; subst
+        | |- ?x = ?y /\ _ =>
+            split
+        | H : ?x = ?y /\ _ |- _ =>
+            destruct H; subst
+        end; try reflexivity).
+        - exists vt. apply wp_bind. revert IHtpb. apply wp_monotone. intro. destruct o. intro. destruct H0. apply wp_ret. subst. intuition.
+        - exists t1. auto.
+  Qed.
 
+  Fixpoint gensem (ctx : list (string * ty)) (expression : expr) (type : ty) : Prop :=
+    match expression with
+    | v_true  => type = ty_bool
+    | v_false => type = ty_bool
+    | e_if cnd coq alt =>
+        gensem ctx cnd ty_bool /\
+        gensem ctx coq type    /\
+        gensem ctx alt type
+    | e_var var =>
+        match (value var ctx) with
+        | None => False
+        | Some t => t = type
+        end
+    | e_app e1 e2 =>
+        exists t2,
+        gensem ctx e1 (ty_func t2 type) /\
+        gensem ctx e2 t2
+    | e_absu var e =>
+        exists t_e t_var,
+        gensem ((var, t_var) :: ctx) e t_e /\
+        type = (ty_func t_var t_e)
+    | e_abst var t_var e =>
+        exists t_e,
+        gensem ((var, t_var) :: ctx) e t_e /\
+        type = (ty_func t_var t_e)
+    end.
+
+  Lemma ex_gensem1 :
+    gensem nil (e_app (e_absu "x" (e_var "x")) v_false) ty_bool.
+  Proof.
+    compute. repeat eexists.
+  Qed.
+
+  Example ex_gensem2 :
+  gensem nil (e_app (e_absu "x" (v_true)) (e_absu "x" (e_var "x"))) ty_bool.
+  Proof.
+    compute. repeat eexists.
+    Unshelve. apply ty_bool.
+  Qed.
+
+End Shallow.
+
+Section Symbolic.
+
+  Inductive Ty (Σ : Ctx nat) : Type :=
+    | Ty_bool : Ty Σ
+    | Ty_func : Ty Σ -> Ty Σ -> Ty Σ
+    | Ty_hole : forall (i : nat), i ∈ Σ -> Ty Σ.
+
+  Definition Env Σ := list (string * Ty Σ).
+
+  Inductive Cstr (A : Ctx nat -> Type) (Σ : Ctx nat) : Type :=
+    | C_eqc : Ty Σ -> Ty Σ -> Cstr A Σ -> Cstr A Σ
+    | C_val : A Σ -> Cstr A Σ
+    | C_fls : Cstr A Σ
+    | C_exi : forall (i : nat), Cstr A (Σ ▻ i) -> Cstr A Σ.
+
+  Check Cstr.
+
+  Check Ty.
+
+  Check Ty_bool.
+
+  Check C_fls Ty.
+
+  (* Adapted from Katamaran: Symbolic/Worlds.v *)
+
+  Inductive Accessibility (Σ₁ : Ctx nat) : Ctx nat -> Type :=
+    | refl    : Accessibility Σ₁ Σ₁
+    | fresh α : forall Σ₂, Accessibility Σ₁ Σ₂ -> Accessibility Σ₁ (Σ₂ ▻ α).
+
+  (* ⊢ A *)
+  Definition Valid (A : Ctx nat -> Type) := forall Σ, A Σ.
+
+  (* A → B *)
+  Definition Impl (A B : Ctx nat -> Type) : Ctx nat -> Type :=
+    fun Σ => (A Σ) -> (B Σ).
+
+  (* □ A *)
+  Definition Box A (Σ : Ctx nat) := forall Σ', Accessibility Σ Σ' -> A Σ'.
+
+  (* _[_] *)
+  Definition Persistent' : Valid (Impl Ty (Box Ty)).
+  Proof. cbv in *. intros. Admitted.
+
+  Definition Persistent_Env : Valid (Impl Env (Box Env)).
+  Admitted.
+
+  Fixpoint Persistent {Σ₁ Σ₂} (t : Ty Σ₁) {w : Accessibility Σ₁ Σ₂} {struct t} : Ty Σ₂.
+  Proof. cbv in *. intros. destruct t eqn:?.
+    - apply Ty_bool.
+    - constructor 2;
+      eapply Persistent. apply t0_1. apply w. apply t0_2. apply w.
+    - constructor 3 with i. admit.
+  Show Proof. (* Defined, not Qed *)
+  Admitted.
+
+  Definition Persistent'' : Valid (Impl Ty (Box Ty)) :=
+    fun w0 x w1 ω01 =>
+      match ω01 with
+      | refl _ => x
+      | fresh _ α Σ _ => Ty_bool (Σ ▻ α)
+      end.
+
+  Definition T {A} := fun (Σ : Ctx nat) (a : Box A Σ) => a Σ (refl Σ).
+
+  Check T.
+
+  Definition trans {Σ₁ Σ₂ Σ₃} (w12 : Accessibility Σ₁ Σ₂) (w23 : Accessibility Σ₂ Σ₃) : Accessibility Σ₁ Σ₃.
+  Proof. induction w23. apply w12. apply fresh. apply IHw23. Defined.
+
+  Definition _4 {A} : Valid (Impl (Box A) (Box (Box A))).
+  Proof. cbv in *. intros.  apply X. eapply trans. apply H. apply H0. Show Proof. Defined.
+
+  Check _4.
+
+  Print Scopes.
+
+  Fixpoint bind [A B] {Σ} (m : Cstr A Σ) (f : Box (Impl A (Cstr B)) Σ) {struct m} : Cstr B Σ.
+  refine (
+    match m with
+    | C_eqc _ _ t1 t2 C1 => _
+    | C_val _ _ v => _
+    | C_fls _ _ => C_fls _ _ (* we just fail *)
+    | C_exi _ _ i C => _
+    end).
+  Proof.
+    - apply C_eqc. apply t1. apply t2. eapply bind.
+      + apply C1.
+      + apply f.
+    - apply T in f. unfold Impl in f. apply f. apply v.
+    - eapply C_exi. eapply bind.
+      + apply C.
+      + apply _4 in f. cbv in *. intros. apply (f _ (fresh _ _ _ (refl Σ)) _ H X).
+  Show Proof.
+  Defined.
+
+  Eval cbv [bind] in @bind.
+
+      Local Notation "[ ω ] x <- ma ;; mb" :=
+        (bind ma (fun _ ω x => mb))
+          (at level 80, x at next level,
+            ma at next level, mb at level 200,
+            right associativity).
+
+  Definition Unit (Σ : Ctx nat) := unit.
+
+  Check Unit.
+
+  Definition assert' {Σ} t1 t2 := C_eqc Unit Σ t1 t2 (C_val Unit Σ tt). (* TODO *)
+
+  Check Persistent_Env.
+
+  (*
+
+  Fixpoint infer'' {Σ} (Γ : Env Σ) (expression : expr) : Cstr Ty Σ :=
+    match expression with
+    | v_true => C_val Ty Σ (Ty_bool Σ)
+    | v_false => C_val Ty Σ (Ty_bool Σ)
+    | e_if cnd coq alt =>
+        [ ω₁ ] t_cnd <- infer'' Γ cnd ;;
+        [ ω₂ ] t_coq <- infer'' ((Persistent_Env _ Γ) _ ω₁) coq ;; (* needs even more PERSISTENCY!!!, find where to persist ω₂ from Σ -> \c0 *)
+        [ ω₃ ] t_alt <- infer'' Γ alt ;; (* TODO: lift Γ into right world *)
+        [ ω₄ ] _ <- assert ((Persistent' _ t_cnd) _ ω₂) (Ty_bool _) ;;
+        [ ω₅ ] _ <- assert (Persistent t_coq) (Persistent t_alt) ;;
+           C_val Ty _ (Persistent t_coq)
+        C_fls Ty _
+    | _ => C_fls Ty Σ
+    end.
+
+  Compute infer' nil (e_if v_true v_true v_false).
+  Compute C_eqc Ty ε (Ty_bool ε) (Ty_bool ε) (C_val Ty ε (Ty_bool ε)).
+
+  *)
 
